\documentclass[11pt, oneside]{article}
\usepackage[margin=1in]{geometry}
\geometry{letterpaper}
\usepackage{amssymb}
\usepackage[fleqn]{amsmath}
\usepackage[sharp]{easylist}
\usepackage{relsize}
\usepackage{graphicx}

\pagenumbering{gobble}              % No page numbering
\setlength{\parindent}{0em}         % No paragraph indenting
\setlength{\parskip}{0.5em}         % Paragraph spacing

\newcommand*{\begineasylist}{\begin{easylist}[itemize]\ListProperties(Style*=$\bullet$\quad, Style2*=\tiny$\blacksquare$\quad, Style3*=$\circ$\quad, Style4*=$\diamond$\quad, FinalSpace=1em, Space=0em, Space*=0em)}

\newcommand*{\begineasylistnumbered}{\begin{easylist}[enumerate]\ListProperties(Numbers=a, Space=0em, Space*=0em)}

\begin{document}

\section*{MSCI 261 Midterm Review (Chpt. 2-5)}

\subsection*{Cash Flow Diagrams}
\begineasylist

\begin{figure}[!ht]
    \centering
    \includegraphics[width=0.7\textwidth]{cash_flow_diagram.png}
\end{figure}

# Cash inflows and outflows are represented by arrows
# Each ``year'' point represents the \emph{\underline{beginning}} of that year

\end{easylist}
\subsection*{Interest}
\begineasylist

# \textbf{Compound interest}: $F = P(1 + i)^N$
## $F$ = future value (value at the end of year N)
## $P$ = present value
## $i$ = interest rate (per period)
## $N$ = number of periods

# \textbf{Simple interest}: $F = PN(1 + i)$

# \textbf{Nominal interest rate}: $i_s$
## ``Normal'' way of stating interest rate
## If annual nominal rate = 12\%/year, then monthly nominal rate = 1\%/month
# \textbf{Effective interest rate}: $i_e$
## ``Actual'' interest rate
## Suppose $i_s$ is stated over a ``small'' period
## Then $i_e$ over a ``large'' period, which consists of $m$ small periods, is
\[ i_e = (1 + i_s)^m - 1 \]
## i.e. effective interest is the rate such that $P(1 + i_s)^m = P(1+i_e)$
# \textbf{Converting nominal annual to effective annual rate}:
\[ i_e = (1 + \frac{i_s}{m})^m - 1 \qquad \text{where $m$ = number of compounding periods in a year} \]
# Continuous compounding -- compounding period is infinitesimally small
\begin{align*}
i_e &= \lim_{m \rightarrow \infty} \Big(1 + \frac{i_s}{m}\Big)^m - 1\\
&= e^{i_s} -1
\end{align*}



\end{easylist}

\end{document}